\documentclass[11pt]{article}
\usepackage{subfigure}
\usepackage{color}
\usepackage{url}
\usepackage{graphicx}
\usepackage{fullpage}
\usepackage[english]{babel}
\usepackage{amssymb}
\usepackage{amsmath}
\usepackage{fancyhdr}
\usepackage{hyperref}
\usepackage{algorithmic}
\usepackage{algorithm}
\usepackage{enumerate}
\usepackage{mdframed}

\DeclareMathOperator*{\argmin}{argmin}
\newcommand*{\argminl}{\argmin\limits}


\begin{document}
\begin{center}
%---------------------------------------------------------------------------------------
%---------------------------------Header------------------------------------------------
%---------------------------------------------------------------------------------------

\framebox{\parbox{6.5in}{
{\bf{STATS 315B: Data Mining, Spring 2016}}\\
{\bf Homework 1, Due 4/28/2016}\\
{\bf Completed by: Henry Neeb, Christopher Kurrus, and Tyler Chase}
}}
\ \\
\end{center}

%---------------------------------------------------------------------------------------
%---------------------------------Answer------------------------------------------------
%---------------------------------------------------------------------------------------

\section*{Problem 9}

\vspace{5 mm}
\noindent
To show that the minimizing values of $\hat{c}_{m}$ are given by $\sum\limits_{i=0}^N (y_{i} I(x_{i} \in R_{m})) / \sum\limits_{i=0}^N (I(x_{i} \in R_{m}))$ we will expand upon our given functions.

\vspace{3 mm}
\noindent
We know our criterion is $\sum\limits_{i=1}^N (y_{i} - F(x_{i}))^2$ and we have $F(x) = \sum\limits_{m=1}^M (c_{m}I(x \in R_{m}))$

\vspace{3 mm}
\noindent
Proceeding, we can expand our criterion into $\sum\limits_{i=1}^N (y_{i} - \sum\limits_{m=1}^M (c_{m}I(x_{i} \in R_{m})))^2$

\vspace{3 mm}
\noindent
Now our goal is to find the minimizing value $min_{c_{m}}[\sum\limits_{i=1}^N (y_{i} - \sum\limits_{m=1}^M (c_{m}I(x_{i} \in R_{m})))^2]$ 

\vspace{3 mm}
\noindent
We will do this using partial differentiation on the $c$ for which $x_{i} \in R_{k}$.  $\frac{d}{dc_{k}}[\sum\limits_{i=1}^N (y_{i} - \sum\limits_{m=1}^M (c_{m}I(x_{i} \in R_{m})))^2] = $

\vspace{3 mm}
\noindent
$\sum\limits_{i=1}^N (2(y_{i} - c_{k})(-I(x_{i} \in R_{k})))$, as the resulting summations over $m$ will all go to zero for $m \neq k$.

\vspace{3 mm}
\noindent
Now we can set equal to zero and eliminate the constant 2, yielding $\sum\limits_{i=1}^N ((y_{i} - c_{k})(-I(x_{i} \in R_{k}))) = 0$

\vspace{3 mm}
\noindent
Distributing and splitting the summation we have $\sum\limits_{i=1}^N (c_{k}I(x_{i} \in R_{k}) - \sum\limits_{i=1}^N (y_{i}I(x_{i} \in R_{k}) = 0$

\vspace{3 mm}
\noindent
So simplifying, ${c}_{k} = \frac{\sum\limits_{i=0}^N (y_{i} I(x_{i} \in R_{k}))}{\sum\limits_{i=0}^N (I(x_{i} \in R_{k}))}$ as desired.

\end{document}