\documentclass[11pt]{article}
\usepackage{subfigure}
\usepackage{color}
\usepackage{url}
\usepackage{graphicx}
\usepackage{fullpage}
\usepackage[english]{babel}
\usepackage{amssymb}
\usepackage{amsmath}
\usepackage{fancyhdr}
\usepackage{hyperref}
\usepackage{algorithmic}
\usepackage{algorithm}
\usepackage{enumerate}
\usepackage{mdframed}


\begin{document}
\begin{center}
%---------------------------------------------------------------------------------------
%---------------------------------Header------------------------------------------------
%---------------------------------------------------------------------------------------

\framebox{\parbox{6.5in}{
{\bf{STATS 315B: Data Mining, Spring 2016}}\\
{\bf Homework 2, Due 5/22/2016}\\
{\bf Completed by: Henry Neeb, Christopher Kurrus, Tyler Chase, and Yash Vyas}
}}
\ \\
\end{center}

%-------------------------------------------------------------------------------
%---------------------------------Answer----------------------------------------
%-------------------------------------------------------------------------------

\section*{Problem 3}

\begin{gather*}
\text{Let } L(y_{i}, a_{0} + \sum_{j = 1}^{n} a_{j}x_{ij}) = L 
\text{ and } a_{0} + \sum_{j = 1}^{n} a_{j}x_{ij} = f(x, a) = f\\
\frac{\partial \hat{R}}{\partial a_{k}} = 
\frac{1}{N} \sum_{j = 1}^{N} \frac{\partial L}{\partial a_{k}}\\
\text{By the chain rule: } 
\frac{\partial L}{\partial a_{k}} = 
\frac{\partial L(y_{i}, f(x, a))}{\partial a_{k}} = 
\frac{\partial L(y_{i}, f(x, a))}{f(x, a)} 
\frac{\partial f(x, a)}{\partial a_{k}} = 
\frac{\partial L}{\partial f} \frac{\partial f}{\partial a_{k}}\\
\frac{\partial f}{\partial a_{k}} = 
\text{Now consider } 
\frac{\partial}{\partial a_{k}} [a_{0} + \sum_{j = 1}^{n} a_{j}x_{ij}]\\
\text{Note that } a_{k} 
\text{ only appears in the sumation and is multiplied by } x_{ik}\\
\text{So all values in } f 
\text{ will evaluate to zero except } a_{k}x_{ik}\\
\text{Then } 
\frac{\partial}{\partial a_{k}} [a_{0} + \sum_{j = 1}^{n} a_{j}x_{ij}] = x_{ik}\\
\text{And } 
\frac{1}{N} \sum_{j = 1}^{N} \frac{\partial L}{\partial a_{k}} = 
\frac{1}{N} \sum_{j = 1}^{N} \frac{\partial L}{\partial f} 
\frac{\partial f}{\partial a_{k}} = 
\frac{1}{N} \sum_{j = 1}^{N} \frac{\partial L}{\partial f} x_{ik}
\end{gather*}

\end{document}